

\\\\
{\omega_1}=  + \frac {\beta}{\left | \beta \right |} \sqrt \frac{\beta+1}{\beta-1}i\omega'
 \ \ \ \ \ \ \ 
{k_1}= +\frac {\beta}{\left | \beta \right |}\sqrt \frac{\beta+1}{\beta-1}i k'
\\
{\omega_2}=  - \frac {\beta}{\left | \beta \right |} \sqrt \frac{\beta+1}{\beta-1}i\omega'
 \ \ \ \ \ \ \
{k_2}= - \frac {\beta}{\left | \beta \right |}\sqrt \frac{\beta+1}{\beta-1}i k'
\\
{\omega_3}=  - \frac {\beta}{\left | \beta \right |} \sqrt \frac{\beta-1}{\beta+1}i\omega'
 \ \ \ \ \ \ \ 
{k_3}= + \frac {\beta}{\left | \beta \right |}\sqrt \frac{\beta-1}{\beta+1}i k'
\\
{\omega_4}=  + \frac {\beta}{\left | \beta \right |} \sqrt \frac{\beta-1}{\beta+1}i\omega'
 \ \ \ \ \ \ \
{k_4}= - \frac {\beta}{\left | \beta \right |}\sqrt \frac{\beta-1}{\beta+1}i k'



\\\\
\\
\beta=\frac {v}{c}, \beta^2\textgreater 1
